src/CSL/BigDynOp.v
@@ -1,0 +1,142 @@
+From iris.algebra Require Export big_op.
+Set Default Proof Using "Type*".
+Local Existing Instances monoid_ne monoid_assoc monoid_comm
+  monoid_left_id monoid_right_id monoid_proper
+  monoid_homomorphism_rel_po monoid_homomorphism_rel_proper
+  monoid_homomorphism_op_proper
+  monoid_homomorphism_ne weak_monoid_homomorphism_proper.
+Require Import EqualDec.
+Require Export SemanticsHelpers.
+
+(* Adapted from the big_op.v files from Iris. Extends those operators to work over DynMaps *)
+
+Definition big_opDM `{Monoid M o} A (Ref Model: A -> Type)
+      (f: ∀ {T}, Ref T → Model T → M) (m: DynMap Ref Model) :=
+  big_opL o (λ _ k, match getDyn m (projT2 k) with
+                    | None => monoid_unit
+                    | Some v => f (projT2 k) v
+                    end) (dynMap_dom m).
+
+(*
+Instance: Params (@big_opDM) 8 := {}.
+*)
+Arguments big_opDM {M} o {_ A Ref Model} _ _ : simpl never.
+Typeclasses Opaque big_opDM.
+Notation "'[^' o 'dmap]' k ↦ x ∈ m , P" := (big_opDM o (λ k x, P) m)
+  (at level 200, o at level 1, m at level 10, k, x at level 1, right associativity,
+   format "[^  o  dmap]  k ↦ x  ∈  m ,  P") : stdpp_scope.
+Notation "'[^' o 'dmap]' x ∈ m , P" := (big_opDM o (λ _ x, P) m)
+  (at level 200, o at level 1, m at level 10, x at level 1, right associativity,
+   format "[^ o  dmap]  x  ∈  m ,  P") : stdpp_scope.
+
+(** ** Big ops over DynMaps *)
+Section DynMap.
+  Context `{Monoid M o}.
+  Infix "`o`" := o (at level 50, left associativity).
+  Context {A : Type} {Ref Model : A → Type}.
+  Context `{dec : EqualDec {x : A & Ref x}}.
+  Implicit Types m : DynMap Ref Model.
+  Implicit Types f g : ∀ {T}, Ref T → Model T → M.
+
+  Lemma big_opDM_forall R f g m :
+    Reflexive R → Proper (R ==> R ==> R) o →
+    (∀ {T} (k: Ref T) x, getDyn m k = Some x → R (f _ k x) (g _ k x)) →
+    R ([^o dmap] k ↦ x ∈ m, f k x) ([^o dmap] k ↦ x ∈ m, g k x).
+  Proof.
+    intros ?? Hf. apply (big_opL_forall R); auto.
+    intros k [i x] ?%elem_of_list_lookup_2.
+    destruct (getDyn) eqn:?; last (exfalso; eapply dynMap_dom_spec); eauto.
+    by apply getDyn_lookup_none.
+  Qed.
+
+  Lemma big_opDM_ext f g m :
+    (∀ {T} (k: Ref T) x, getDyn m k = Some x → f _ k x = g _ k x) →
+    ([^o dmap] k ↦ x ∈ m, f k x) = ([^o dmap] k ↦ x ∈ m, g k x).
+  Proof. apply big_opDM_forall; apply _. Qed.
+  Lemma big_opDM_proper f g m :
+    (∀ {T} (k: Ref T) x, getDyn m k = Some x → f _ k x ≡ g _ k x) →
+    ([^o dmap] k ↦ x ∈ m, f k x) ≡ ([^o dmap] k ↦ x ∈ m, g k x).
+  Proof. apply big_opDM_forall; apply _. Qed.
+  Lemma big_opDM_proper_map f m1 m2 :
+    m1 ≡ m2 →
+    ([^o dmap] k ↦ x ∈ m1, f k x) ≡ ([^o dmap] k ↦ x ∈ m2, f k x).
+  Proof.
+    intros Hequiv. unfold big_opDM.
+    rewrite big_opL_permutation; last by (rewrite Hequiv; reflexivity).
+    eapply big_opL_proper => ???.
+    by rewrite Hequiv.
+  Qed.
+
+  Global Instance big_opDM_ne n :
+    Proper (forall_relation (λ T, pointwise_relation (Ref T) (pointwise_relation (Model T) (dist n)))
+                            ==> eq ==> dist n)
+           (big_opDM o (A:=A) (Ref:=Ref) (Model:=Model)).
+  Proof. intros f g Hf m ? <-. apply big_opDM_forall; apply _ || intros; apply Hf. Qed.
+  Global Instance big_opDM_proper' :
+    Proper (forall_relation (λ T, pointwise_relation (Ref T) (pointwise_relation (Model T) (≡)))
+                            ==> (≡) ==> (≡))
+           (big_opDM o (A:=A) (Ref:=Ref) (Model:=Model)).
+  Proof.
+    intros f g Hf m1 m2 Hequiv.
+    rewrite big_opDM_proper_map //.
+    apply big_opDM_forall; apply _ || intros; apply Hf.
+  Qed.
+  Global Instance big_opDM_proper'' :
+    Proper (eq ==> (≡) ==> (≡))
+           (big_opDM o (A:=A) (Ref:=Ref) (Model:=Model)).
+  Proof. intros ?? <- ?? ?. eapply big_opDM_proper'; eauto. intros ??. reflexivity. Qed.
+
+  Lemma big_opDM_empty f : ([^o dmap] k↦x ∈ (∅ : DynMap Ref Model), f k x) = monoid_unit.
+  Proof. rewrite /big_opDM //=. Qed.
+
+  Lemma big_opDM_updDyn {T} f m (i: Ref T) (x: Model T):
+    getDyn m i = None →
+    ([^o dmap] k↦y ∈ updDyn (dec := dec) i x m, f k y) ≡ f _ i x `o` [^o dmap] k↦y ∈ m, f k y.
+  Proof.
+    intros Hnone. rewrite /big_opDM //= decide_False //= ?getDyn_updDyn //=; last first.
+    { rewrite -dynMap_dom_spec => Hfalse. by apply Hfalse, getDyn_lookup_none. }
+    f_equiv. apply big_opL_proper => k y. intros Hlookup%elem_of_list_lookup_2.
+    rewrite getDyn_updDyn_ne1 //.
+    intros Heq. subst. apply dynMap_dom_spec in Hlookup. apply Hlookup.
+    by apply getDyn_lookup_none.
+  Qed.
+
+  Lemma big_opDM_delete {T} f m (i: Ref T) x :
+    getDyn m i = Some x →
+    ([^o dmap] k↦y ∈ m, f k y) ≡ f _ i x `o` [^o dmap] k↦y ∈ deleteDyn (dec := dec) i m, f k y.
+  Proof.
+    rewrite -big_opDM_updDyn ?getDyn_deleteDyn // => Hsome.
+    by rewrite updDyn_deleteDyn updDyn_identity.
+  Qed.
+
+  Lemma big_opM_singleton {T} f (i: Ref T) x :
+    ([^o dmap] k↦y ∈ updDyn (dec := dec) i x ∅, f k y) ≡ f _ i x.
+  Proof.
+    rewrite big_opDM_updDyn/=; last auto using lookup_empty.
+    by rewrite big_opDM_empty right_id.
+  Qed.
+
+  Lemma big_opDM_unit m : ([^o dmap] k↦y ∈ m, (λ _ _ _, monoid_unit) k y) ≡ (monoid_unit : M).
+  Proof.
+    etransitivity; last eapply big_opL_unit.
+    unfold big_opDM. eapply big_opL_proper.
+    intros ??; by destruct getDyn.
+  Qed.
+
+  Lemma big_opM_insert_override {T} f m (i: Ref T) x x' :
+    getDyn m i = Some x → f _ i x ≡ f _ i x' →
+    ([^o dmap] k↦y ∈ updDyn (dec := dec) i x' m, f k y) ≡ ([^o dmap] k↦y ∈ m, f k y).
+  Proof.
+    intros ? Hx. rewrite -updDyn_deleteDyn big_opDM_updDyn ?getDyn_deleteDyn //.
+    by rewrite -Hx -big_opDM_delete.
+  Qed.
+
+  Lemma big_opM_opM f g m :
+    ([^o dmap] k↦x ∈ m, (λ _ k x, f _ k x `o` g _ k x) k x )
+    ≡ ([^o dmap] k↦x ∈ m, f k x) `o` ([^o dmap] k↦x ∈ m, g k x).
+  Proof.
+    rewrite /big_opM -big_opL_opL. eapply big_opL_proper => k [??] Heq.
+    destruct (getDyn) => //=. by rewrite right_id.
+  Qed.
+End DynMap.
+
